theories/Syntax/ListNat.v
@@ -1,0 +1,81 @@
+From Cyclic.Syntax Require Import StrictPos Term Examples.
+
+From Stdlib Require Import List.
+
+From Cyclic.Syntax Require Import StrictPos Term Examples.
+
+Import ListNotations.
+Import Term.Syntax.
+
+Set Default Proof Using "Type".
+
+Module ListNat.
+
+  (** We assume [Nat] is inductive 0 (from [Syntax.Examples]).
+      We define [List Nat] as inductive 1. *)
+
+  Definition list_ty : tm := tInd 1 [].
+
+  Definition List_sig : ind_sig tm := {|
+    ind_params := [];
+    ind_indices := [];
+    ind_level := 0;
+    ind_ctors := [
+      {| ctor_param_tys := []; ctor_rec_args := []; ctor_indices := [] |};
+      {| ctor_param_tys := [Examples.nat_ty]; ctor_rec_args := [[]]; ctor_indices := [] |}
+    ]
+  |}.
+
+  Definition nil : tm := tRoll 1 0 [].
+  Definition cons (x xs : tm) : tm := tRoll 1 1 [x; xs].
+
+  (** A simple function type [Nat -> Nat]. *)
+  Definition nat2nat : tm := tPi Examples.nat_ty Examples.nat_ty.
+
+  (** map : (Nat -> Nat) -> List -> List *)
+  Definition map_ty : tm := tPi nat2nat (tPi list_ty list_ty).
+
+  Definition map_body : tm :=
+    (* self : map_ty *)
+    tLam nat2nat ( (* f : Nat -> Nat *)
+      tLam list_ty ( (* l : List *)
+        tCase 1 (tVar 0) list_ty
+          [ nil;
+            (* cons branch: \x:Nat. \xs:List. cons (f x) (map f xs) *)
+            tLam Examples.nat_ty (
+              tLam list_ty (
+                cons
+                  (tApp (tVar 3) (tVar 1))
+                  (tApp (tApp (tVar 4) (tVar 3)) (tVar 0))
+              ))
+          ]
+      )).
+
+  Definition map : tm := tFix map_ty map_body.
+
+  (** length : List -> Nat *)
+  Definition length_ty : tm := tPi list_ty Examples.nat_ty.
+
+  Definition length_body : tm :=
+    (* self : length_ty *)
+    tLam list_ty (
+      tCase 1 (tVar 0) Examples.nat_ty
+        [ Examples.zero;
+          (* cons branch: \x:Nat. \xs:List. succ (length xs) *)
+          tLam Examples.nat_ty (
+            tLam list_ty (
+              Examples.succ (tApp (tVar 3) (tVar 0))
+            ))
+        ]
+    ).
+
+  Definition length : tm := tFix length_ty length_body.
+
+  (** Convenience: list notation in the object language. *)
+  Fixpoint list_lit (xs : list tm) : tm :=
+    match xs with
+    | [] => nil
+    | x :: xs => cons x (list_lit xs)
+    end.
+
+End ListNat.
